Remove references to δP in semantics and proofs (#96)
The existence and use of the `HasBool` class makes it unnecessary, and
it was always a little messy.

By submitting this pull request, I confirm that you can use, modify,
copy, and redistribute this contribution, under the terms of your
choice.

---------

Co-authored-by: Shilpi Goel <shigoel@gmail.com>

Strata/DL/Imperative/CmdSemantics.lean
@@ -33,7 +33,7 @@ Evaluation relation of an Imperative command `Cmd`.
 -/
 -- (FIXME) Change to a type class?
 abbrev EvalCmdParam (P : PureExpr) (Cmd : Type) :=
-  SemanticEval P → SemanticEvalBool P → SemanticStore P → SemanticStore P → Cmd →
+  SemanticEval P → SemanticStore P → SemanticStore P → Cmd →
   SemanticStore P → Prop
 
 /-- ### Well-Formedness of `SemanticStore`s -/
@@ -218,11 +218,10 @@ theorem invStoresExceptComm :
 -- or that when δ evaluates to none, δP evaluates to False
   -/
 def WellFormedSemanticEvalBool {P : PureExpr} [HasBool P] [HasBoolNeg P]
-    (δ : SemanticEval P) (δP : SemanticEvalBool P) : Prop :=
-    ∀ σ₀ σ e b,
-      (δ σ₀ σ e = some Imperative.HasBool.tt ↔ δP σ₀ σ e = (some true)) ∧
-      (δ σ₀ σ e = some Imperative.HasBool.ff ↔ δP σ₀ σ e = (some false)) ∧
-      (δP σ₀ σ e = (some b) ↔ δP σ₀ σ (Imperative.HasBoolNeg.neg e) = (some (not b)))
+    (δ : SemanticEval P) : Prop :=
+    ∀ σ₀ σ e,
+      (δ σ₀ σ e = some Imperative.HasBool.tt ↔ δ σ₀ σ (Imperative.HasBoolNeg.neg e) = (some HasBool.ff)) ∧
+      (δ σ₀ σ e = some Imperative.HasBool.ff ↔ δ σ₀ σ (Imperative.HasBoolNeg.neg e) = (some HasBool.tt))
 
 def WellFormedSemanticEvalVal {P : PureExpr} [HasVal P]
     (δ : SemanticEval P) : Prop :=
@@ -261,40 +260,38 @@ An inductively-defined operational semantics that depends on
 environment lookup and evaluation functions for expressions.
 -/
 inductive EvalCmd [HasFvar P] [HasBool P] [HasBoolNeg P] :
-  SemanticEval P → SemanticEvalBool P →
-  SemanticStore P → SemanticStore P →
-  Cmd P → SemanticStore P → Prop where
+  SemanticEval P → SemanticStore P → SemanticStore P → Cmd P → SemanticStore P → Prop where
   | eval_init :
     δ σ₀ σ e = .some v →
     InitState P σ x v σ' →
     WellFormedSemanticEvalVar δ →
     ---
-    EvalCmd δ δP σ₀ σ (.init x _ e _) σ'
+    EvalCmd δ σ₀ σ (.init x _ e _) σ'
 
   | eval_set :
     δ σ₀ σ e = .some v →
     UpdateState P σ x v σ' →
     WellFormedSemanticEvalVar δ →
     ----
-    EvalCmd δ δP σ₀ σ (.set x e _) σ'
+    EvalCmd δ σ₀ σ (.set x e _) σ'
 
   | eval_havoc :
     UpdateState P σ x v σ' →
     WellFormedSemanticEvalVar δ →
     ----
-    EvalCmd δ δP σ₀ σ (.havoc x _) σ'
+    EvalCmd δ σ₀ σ (.havoc x _) σ'
 
   | eval_assert :
-    δP σ₀ σ e = .some true →
-    WellFormedSemanticEvalBool δ δP →
+    δ σ₀ σ e = .some HasBool.tt →
+    WellFormedSemanticEvalBool δ →
     ----
-    EvalCmd δ δP σ₀ σ (.assert _ e _) σ
+    EvalCmd δ σ₀ σ (.assert _ e _) σ
 
   | eval_assume :
-    δP σ₀ σ e = .some true →
-    WellFormedSemanticEvalBool δ δP →
+    δ σ₀ σ e = .some HasBool.tt →
+    WellFormedSemanticEvalBool δ →
     ----
-    EvalCmd δ δP σ₀ σ (.assume _ e _) σ
+    EvalCmd δ σ₀ σ (.assume _ e _) σ
 
 end section
 
